translations now compile (or almost)

translations/translation_utils.v
@@ -1,13 +1,16 @@
-Require Import Template.Ast Template.Typing Template.Checker.
+Require Import Template.Ast Template.Typing Template.Checker Template.monad_utils Template.Template.
+Require Import Translations.sigma.
 Require Import List.
-Import ListNotations String.
+Import ListNotations MonadNotation String.
 Open Scope string_scope.
 
-Inductive global_reference :=
-(* VarRef of Names.variable *)
-  | ConstRef : string (* kername *) -> global_reference
-  | IndRef : inductive -> global_reference
-  | ConstructRef : inductive -> nat -> global_reference.
+Axiom todo : forall {A}, A.
+
+(* Inductive global_reference := *)
+(* (* VarRef of Names.variable *) *)
+(*   | ConstRef : string (* kername *) -> global_reference *)
+(*   | IndRef : inductive -> global_reference *)
+(*   | ConstructRef : inductive -> nat -> global_reference. *)
 
 Hint Resolve String.string_dec Peano_dec.eq_nat_dec : eq_dec.
 
@@ -27,48 +30,28 @@ Definition gref_eq_dec
   decide equality; eauto with eq_dec.
 Defined.
 
-Definition tsl_context := list (global_reference * term).
+Definition tsl_table := list (global_reference * term).
 
 Definition empty_global_ctx : global_context := [].
-Definition empty_tsl_ctx : tsl_context := [].
+Definition empty_tsl_table : tsl_table := [].
 
 Definition add_global_ctx : global_decl -> global_context -> global_context
   := cons.
-Definition add_tsl_ctx : global_reference -> term -> tsl_context -> tsl_context
+Definition add_tsl_table : global_reference -> term -> tsl_table -> tsl_table
   := fun kn t => cons (kn, t).
 
 
-Fixpoint lookup_tsl_ctx (E : tsl_context) (gr : global_reference)
+Fixpoint lookup_tsl_table (E : tsl_table) (gr : global_reference)
   : option term :=
   match E with
   | nil => None
   | hd :: tl =>
     if gref_eq_dec gr (fst hd) then Some (snd hd)
-    else lookup_tsl_ctx tl gr
+    else lookup_tsl_table tl gr
   end.
 
 
-Section MonadOperations.
-  Import MonadNotation.
-  Context {T} {M : Monad T}.
-
-  Fixpoint monad_map {A B} (f : A -> T B) (l : list A)
-    : T (list B)
-    := match l with
-       | nil => ret nil
-       | x :: l => x' <- f x ;;
-                  l' <- monad_map f l ;;
-                  ret (x' :: l')
-       end.
-
-  Fixpoint monad_fold_left {A B} (f : A -> B -> T A) (l : list B) (x : A)
-    : T A
-    := match l with
-       | nil => ret x
-       | y :: l => x' <- f x y ;;
-                     monad_fold_left f l x'
-       end.
-End MonadOperations.
+Definition tsl_context := (global_context * tsl_table)%type.
 
 
 Inductive tsl_error :=
@@ -81,32 +64,37 @@ Inductive tsl_result A :=
 | Success : A -> tsl_result A
 | Error : tsl_error -> tsl_result A.
 
+Arguments Success {_} _.
+Arguments Error {_} _.
+
 Instance tsl_monad : Monad tsl_result :=
-  {| ret A a := Success A a ;
+  {| ret A a := Success a ;
      bind A B m f :=
        match m with
-       | Success _ a => f a
-       | Error _ e => Error _ e
+       | Success a => f a
+       | Error e => Error e
        end
   |}.
 
 Instance monad_exc : MonadExc tsl_error tsl_result :=
-  { raise A e := Error A e;
+  { raise A e := Error e;
     catch A m f :=
       match m with
-      | Success _ a => m
-      | Error _ t => f t
+      | Success a => m
+      | Error t => f t
       end
   }.
 
 
 
-Class Translation := { tsl_tm : global_context -> tsl_context -> term -> tsl_result term }.
+Class Translation := { tsl_id : ident -> ident ;
+                       tsl_tm : tsl_context -> term -> tsl_result term ;
+                       tsl_ty : tsl_context -> term -> tsl_result term ;
+                       tsl_ind : tsl_context -> ident -> mutual_inductive_entry
+                            -> tsl_result (tsl_table * list mutual_inductive_entry)
+                     }.
 
-Class TranslationType := { tsl_typ : global_context -> tsl_context -> term -> tsl_result term }.
 
-
-Require Import Template.Template Translations.sigma.
 
 Quote Definition tSigma := sigma.
 Quote Definition tPair := @mk_sig.
@@ -115,14 +103,212 @@ Definition pair (typ1 typ2 t1 t2 : term) : term
 Definition pack (t u : term) : term
   := tApp tSigma [ t ; u ].
 Definition proj1 (t : term) : term
-  := tProj (mkInd "Template.sigma.sigma" 0, 2, 0) t.
+  := tProj (mkInd "Translations.sigma.sigma" 0, 2, 0) t.
 Definition proj2 (t : term) : term
-  := tProj (mkInd "Template.sigma.sigma" 0, 2, 1) t.
+  := tProj (mkInd "Translations.sigma.sigma" 0, 2, 1) t.
 Definition proj (b : bool) (t : term) : term
-  := tProj (mkInd "Template.sigma.sigma" 0, 2, if b then 0 else 1) t.
+  := tProj (mkInd "Translations.sigma.sigma" 0, 2, if b then 0 else 1) t.
 
 Quote Definition tBool := bool.
 Quote Definition tTrue := true.
 Definition timesBool (t : term) :=
   tApp tSigma [t; tLambda nAnon t tBool].
 Definition pairTrue typ t := pair typ (tLambda nAnon typ tBool) t tTrue.
+
+Definition tsl_ident (id : ident) : ident := (id ++ "ᵗ")%string.
+
+Definition print_nf {A} (msg : A) : TemplateMonad unit
+  := (tmEval all msg) >>= tmPrint.
+
+Definition tTranslate (tsl : Translation) (ΣE : tsl_context) (id : ident)
+  : TemplateMonad (option tsl_context) :=
+  gr <- tmAbout id ;;
+  match gr with
+  | IndRef ind
+  | ConstructRef ind _ => tmPrint "todo tTranslate" ;; ret None
+  | ConstRef kn =>
+    e <- tmQuoteConstant kn true ;;
+    print_nf ("toto1" ++ id) ;;
+    match e with
+    | ParameterEntry _ => print_nf (id ++ "is an axiom, not a definition") ;;
+                         ret None
+    | DefinitionEntry {| definition_entry_type := A;
+                         definition_entry_body := t |} =>
+      print_nf ("toto2 " ++ id) ;;
+      tmPrint t ;;
+      match tsl_tm ΣE t with
+      | Error e => tmPrint "tsl error in term: " ;; tmPrint e ;; ret None
+      | Success t' =>
+        print_nf ("toto3 " ++ id) ;;
+        match tsl_ty ΣE A with
+        | Error e => tmPrint "tsl error in type: " ;; tmPrint e ;; ret None
+        | Success A' =>
+          print_nf ("toto4 " ++ id) ;;
+          id' <- tmEval all (tsl_id id) ;;
+          tmMkDefinition id' t' ;;
+          print_nf ("toto5 " ++ id) ;;
+          let decl := {| cst_universes := [];
+                         cst_type := A; cst_body := Some t |} in
+          let Σ' := ConstantDecl kn decl :: (fst ΣE) in
+          let E' := (ConstRef kn, tConst id' []) :: (snd ΣE) in
+          print_nf  (id ++ " has been translated as " ++ id') ;;
+          tmEval all (Some (Σ', E'))
+        end
+      end
+    end
+  end.
+
+
+
+Definition tImplement (tsl : Translation) (ΣE : tsl_context)
+           (id : ident) (A : Type)
+  : TemplateMonad (option tsl_context) :=
+  tA <- tmQuote A ;;
+  match tsl_ty ΣE tA with
+  | Error e => tmPrint "tsl error in type" ;; tmPrint e ;;
+                tmReturn None
+  | Success tA' =>
+    id' <- tmEval all (tsl_id id) ;;
+    A' <- tmUnquoteTyped Type tA' ;;
+    tmLemma id' A' ;;
+    tmAxiom id A ;;
+    let decl := {| cst_universes := [];
+                   cst_type := tA; cst_body := None |} in
+    let Σ' := ConstantDecl id decl :: (fst ΣE) in (* should be kn *)
+    let E' := (ConstRef id, tConst id' []) :: (snd ΣE) in (* id or kn ?? *)
+    print_nf (id ++ " has been translated as " ++ id') ;;
+    tmEval all (Some (Σ', E'))
+  end.
+
+
+Definition tImplementExisting (tsl_id : ident -> ident)
+           (tsl_tm tsl_ty : global_context -> tsl_table -> term
+                            -> tsl_result term)
+           (Σ : tsl_context) (id : ident)
+  : TemplateMonad (option tsl_context) :=
+  e <- tmQuoteConstant id true ;;
+  match e with
+  | ParameterEntry _ => tmPrint "Not a definition" ;;
+                       tmReturn None
+  | DefinitionEntry {| definition_entry_type := A;
+                       definition_entry_body := t |} =>
+    match tsl_ty (fst Σ) (snd Σ) A with
+    | Error _ => tmPrint "tsl error in type" ;;
+                  tmReturn None
+    | Success tA' =>
+      id' <- tmEval all (tsl_id id) ;;
+      A' <- tmUnquoteTyped Type tA' ;;
+      tmLemma id' A' ;;
+      let decl := {| cst_universes := [];
+                     cst_type := A; cst_body := Some t |} in
+      let Σ' := ConstantDecl id decl :: (fst Σ) in
+      let E' := (ConstRef id, tConst id' []) :: (snd Σ) in
+      msg <- tmEval all (id ++ " has been translated as " ++ id') ;;
+      tmPrint msg ;;
+      tmReturn (Some (Σ', E'))
+    end
+  end.
+
+
+
+Fixpoint extract_mind_decl_from_program (id : ident) (p : program)
+  : option minductive_decl
+  := match p with
+     | PConstr _ _ _ _ p => extract_mind_decl_from_program id p
+     | PType id' n inds p => if string_dec id id' then
+                              Some (Build_minductive_decl n inds)
+                            else extract_mind_decl_from_program id p
+     | PAxiom _ _ _ p => extract_mind_decl_from_program id p
+     | PIn _ => None
+     end.
+
+Fixpoint decompose_prod (t : term) : (list name) * (list term) * term :=
+  match t with
+  | tProd n A B => let (nAs, B) := decompose_prod B in
+                  let (ns, As) := nAs in
+                  (n :: ns, A :: As, B)
+  | _ => ([], [], t)
+  end.
+
+Definition get_ident (n : name) :=
+  match n with
+  | nAnon => "XX"
+  | nNamed i => i
+  end.
+
+Fixpoint remove_arity (n : nat) (t : term) : term :=
+  match n with
+  | O => t
+  | S n => match t with
+          | tProd _ _ B => remove_arity n B
+          | _ => t (* todo *)
+          end
+  end.
+
+Definition option_get {A} (default : A) (x : option A) : A
+  := match x with
+     | Some x => x
+     | None => default
+     end.
+
+Definition mind_decl_to_entry (* (id : ident) *) (decl : minductive_decl)
+  : mutual_inductive_entry.
+Proof.
+  refine ({|
+             mind_entry_record := None; (* not a record *)
+             mind_entry_finite := Finite; (* inductive *)
+             mind_entry_params := _;
+             mind_entry_inds := _;
+             mind_entry_polymorphic := false;
+             mind_entry_private := None;
+           |}).
+  - refine (match List.hd_error decl.(ind_bodies) with
+            | Some i0 => _
+            | None => nil (* todo *)
+            end).
+    pose (typ := decompose_prod i0.(ind_type)).
+    destruct typ as [[names types] _].
+    apply (List.firstn decl.(ind_npars)) in names.
+    apply (List.firstn decl.(ind_npars)) in types.
+    refine (List.rev (List.combine _ _)).
+    exact (List.map get_ident names).
+    exact (List.map LocalAssum types).
+    (* pose (fold_left_i (fun acc i ty => let na := tVar (get_ident (List.nth i names nAnon)) *)
+    (*                                 in (na :: fst acc, substl (fst acc) ty :: snd acc)) types ([], [])). *)
+    (* exact (snd p). *)
+  - refine (List.map _ decl.(ind_bodies)).
+    intros [].
+    refine ({| mind_entry_typename := ind_name;
+               mind_entry_arity := remove_arity decl.(ind_npars) ind_type;
+               mind_entry_template := false;
+               mind_entry_consnames := _;
+               mind_entry_lc := _;
+            |}).
+    
+    refine (List.map (fun x => fst (fst x)) ind_ctors).
+    refine (List.map (fun x => remove_arity decl.(ind_npars)
+                                                (snd (fst x))) ind_ctors).
+Defined.
+
+(* Inductive eq' (A : Set) (x : A) : A -> Prop :=  eq_refl' : eq' A x x. *)
+(* Quote Recursively Definition eq'_prog := eq'. *)
+(* Definition eq'_decl := Eval compute in *)
+(*       extract_mind_decl_from_program "Top.eq'" eq'_prog. *)
+
+Quote Recursively Definition sigma_prog := @sigma.
+Quote Recursively Definition eq_prog := @eq.
+Quote Recursively Definition nat_prog := nat.
+
+Definition eq_decl := Eval compute in
+      option_get todo (extract_mind_decl_from_program "Coq.Init.Logic.eq" eq_prog).
+Definition sigma_decl := Eval compute in
+      option_get todo (extract_mind_decl_from_program "Template.sigma.sigma" sigma_prog).
+Definition nat_decl := Eval compute in
+      option_get todo (extract_mind_decl_from_program "Coq.Init.Datatypes.nat" nat_prog).
+
+Definition eq_entry := Eval compute in mind_decl_to_entry eq_decl.
+Definition sigma_entry := Eval compute in mind_decl_to_entry sigma_decl.
+Definition nat_entry := Eval compute in mind_decl_to_entry nat_decl.
+(* Make Inductive eq_entry. *)
+(* Make Inductive sigma_entry. *)
+
