translations/tsl_param.v
@@ -1,15 +1,16 @@
-Require Import Template.Template Template.Ast Translations.sigma.
+(* -*- coq-prog-args: ("-type-in-type" "-top" "Translations.tsl_param") -*-  *)
+Require Import Template.Template Template.Ast Template.monad_utils Translations.sigma.
 Require Import Template.Induction Template.LiftSubst Template.Typing Template.Checker.
 Require Import  Translations.translation_utils.
 Import String Lists.List.ListNotations MonadNotation.
-Open Scope list_scope. Open Scope string_scope.
+Open Scope list_scope. Open Scope string_scope. Open Scope sigma_scope.
 
 
-Reserved Notation "'tsl_ty'".
+Reserved Notation "'tsl_ty_param'".
 
 
 (* if b it is the first translation, else the second *)
-Fixpoint tsl_rec (fuel : nat) (Σ : global_context) (E : tsl_context) (Γ : context) (b : bool) (t : term) {struct fuel}
+Fixpoint tsl_rec (fuel : nat) (Σ : global_context) (E : tsl_table) (Γ : context) (b : bool) (t : term) {struct fuel}
   : tsl_result term :=
   match fuel with
   | O => raise NotEnoughFuel
@@ -28,35 +29,35 @@ Fixpoint tsl_rec (fuel : nat) (Σ : global_context) (E : tsl_context) (Γ : cont
                     A2 <- tsl_rec fuel Σ E Γ false A ;;
                     ret (tCast t2 c (tApp A2 [t1]))
   | tProd n A B => if b then
-                    A' <- tsl_ty fuel Σ E Γ A ;;
+                    A' <- tsl_ty_param fuel Σ E Γ A ;;
                     B1 <- tsl_rec fuel Σ E (Γ ,, vass n A) true B ;;
                     ret (tProd n A' B1)
                   else
-                    A' <- tsl_ty fuel Σ E Γ A ;;
+                    A' <- tsl_ty_param fuel Σ E Γ A ;;
                     B1 <- tsl_rec fuel Σ E (Γ ,, vass n A) true B ;;
                     B2 <- tsl_rec fuel Σ E (Γ ,, vass n A) false B ;;
                     ret (tLambda (nNamed "f") (tProd n A' B1)
                                  (tProd n (lift 1 0 A')
                                         (tApp (lift 1 1 B2)
                                               [tApp (tRel 1) [tRel 0]])))
-  | tLambda n A t => A' <- tsl_ty fuel Σ E Γ A ;;
+  | tLambda n A t => A' <- tsl_ty_param fuel Σ E Γ A ;;
                     t' <- tsl_rec fuel Σ E (Γ ,, vass n A) b t ;;
                     ret (tLambda n A' t')
   | tLetIn n t A u => t' <- tsl_term fuel Σ E Γ t ;;
-                     A' <- tsl_ty fuel Σ E Γ A ;;
+                     A' <- tsl_ty_param fuel Σ E Γ A ;;
                      u' <- tsl_rec fuel Σ E (Γ ,, vdef n t A) b u ;;
                      ret (tLetIn n t' A' u')
   | tApp t u => t' <- tsl_rec fuel Σ E Γ b t ;;
                u' <- monad_map (tsl_term fuel Σ E Γ) u ;;
                ret (tApp t' u')
-  | tConst _ as t
-  | tInd _ as t
-  | tConstruct _ _ as t => t' <- tsl_term fuel Σ E Γ t ;;
-                          ret (proj b t')
+  | tConst _ _ as t
+  | tInd _ _ as t
+  | tConstruct _ _ _ as t => t' <- tsl_term fuel Σ E Γ t ;;
+                            ret (proj b t')
   | _ => raise TranslationNotHandeled
   end
   end
-with tsl_term  (fuel : nat) (Σ : global_context) (E : tsl_context) (Γ : context) (t : term) {struct fuel}
+with tsl_term  (fuel : nat) (Σ : global_context) (E : tsl_table) (Γ : context) (t : term) {struct fuel}
   : tsl_result term :=
   match fuel with
   | O => raise NotEnoughFuel
@@ -64,20 +65,21 @@ with tsl_term  (fuel : nat) (Σ : global_context) (E : tsl_context) (Γ : contex
   match t with
   | tRel n => ret (tRel n)
   | tCast t c A => t' <- tsl_term fuel Σ E Γ t ;;
-                  A' <- tsl_ty fuel Σ E Γ A ;;
+                  A' <- tsl_ty_param fuel Σ E Γ A ;;
                   ret (tCast t' c A')
-  | tConst s => match lookup_tsl_ctx E (ConstRef s) with
-               | Some t => ret t
-               | None => raise (TranslationNotFound s)
-               end
-  | tInd i =>
-    match lookup_tsl_ctx E (IndRef i) with
+  | tConst s univs =>
+    match lookup_tsl_table E (ConstRef s) with
+    | Some t => ret t
+    | None => raise (TranslationNotFound s)
+    end
+  | tInd i univs =>
+    match lookup_tsl_table E (IndRef i) with
     | Some t => ret t
     | None => raise (TranslationNotFound (string_of_gref (IndRef i)))
     end
-  | tConstruct i n =>
-    match lookup_tsl_ctx E (ConstructRef i n) with
-    | Some decl => raise TranslationNotHandeled
+  | tConstruct i n univs =>
+    match lookup_tsl_table E (ConstructRef i n) with
+    | Some t => ret t
     | None => raise (TranslationNotFound (string_of_gref (ConstructRef i n)))
     end
   | t => match infer Σ Γ t with
@@ -90,13 +92,13 @@ with tsl_term  (fuel : nat) (Σ : global_context) (E : tsl_context) (Γ : contex
         end
   end
   end
-where "'tsl_ty'" := (fun fuel Σ E Γ t =>
+where "'tsl_ty_param'" := (fun fuel Σ E Γ t =>
                         t1 <- tsl_rec fuel Σ E Γ true t ;;
                         t2 <- tsl_rec fuel Σ E Γ false t ;;
                         ret (pack t1 t2)).
 
 
-(* Fixpoint tsl_rec (Σ : global_context) (E : tsl_context) (Γ : context) (b : bool) (t : term) {struct t} *)
+(* Fixpoint tsl_rec (Σ : global_context) (E : tsl_table) (Γ : context) (b : bool) (t : term) {struct t} *)
 (*   : tsl_result term := *)
 (*   match t with *)
 (*   | tRel n => ret (proj b (tRel n)) *)
@@ -139,7 +141,7 @@ where "'tsl_ty'" := (fun fuel Σ E Γ t =>
 (*                           ret (proj b t') *)
 (*   | _ => raise TranslationNotHandeled *)
 (*   end *)
-(* with tsl_term (Σ : global_context) (E : tsl_context) (Γ : context) (t : term) {struct t} *)
+(* with tsl_term (Σ : global_context) (E : tsl_table) (Γ : context) (t : term) {struct t} *)
 (*   : tsl_result term := *)
 (*   match t with *)
 (*   | tRel n => ret (tRel n) *)
@@ -147,7 +149,7 @@ where "'tsl_ty'" := (fun fuel Σ E Γ t =>
 (*                   A' <- tsl_typ Σ E Γ A ;; *)
 (*                   ret (tCast t' c A') *)
 (*   | tConst s *)
-(*   | tInd (mkInd s _) => match lookup_tsl_ctx E s with *)
+(*   | tInd (mkInd s _) => match lookup_tsl_table E s with *)
 (*                        | Some t => ret (tConst t) *)
 (*                        | None => raise (TranslationNotFound s) *)
 (*                        end *)
@@ -174,8 +176,213 @@ where "'tsl_ty'" := (fun fuel Σ E Γ t =>
 
 
 
-Instance tsl_param_instance_term : Translation
-  := {| tsl_tm := fun Σ E => tsl_term fuel Σ E [] |}.
+Instance tsl_param : Translation
+  := {| tsl_id := tsl_ident ;
+        tsl_tm := fun ΣE => tsl_term fuel (fst ΣE) (snd ΣE) [] ;
+        tsl_ty := fun ΣE => tsl_ty_param fuel (fst ΣE) (snd ΣE) [] ;
+        tsl_ind := todo |}.
 
-Instance tsl_param_instance_type : TranslationType
-  := {| tsl_typ := fun Σ E => tsl_ty fuel Σ E [] |}.
+
+Definition TslParam := tTranslate tsl_param.
+Definition ImplParam := tImplement tsl_param.
+(* Definition ImplEParam := tImplementExisting tsl_ident tsl_tm tsl_ty_param. *)
+
+Notation "'TYPE'" := (exists A, A -> Type).
+Notation "'El' A" := (sigma (π1 A) (π2 A)) (at level 20).
+
+Definition Ty := Type.
+Run TemplateProgram (TslParam ([],[]) "Ty" >>= tmPrint).
+Check Tyᵗ : El Tyᵗ.
+
+(* Definition Tyᵗ : El Tyᵗ := *)
+(*   @mk_sig Type (fun A => A -> Type) Type (fun A => A -> Type). *)
+
+Definition mkTYPE (A₀ : Type) (Aᴿ : A₀ -> Type) : El Tyᵗ :=
+  @mk_sig Type (fun A₀ => A₀ -> Type) A₀ Aᴿ.
+
+Definition Prodᶠ (A : El Tyᵗ) (B : El A -> El Tyᵗ) : El Tyᵗ :=
+  mkTYPE
+    (forall x : El A, (B x).1)
+    (fun f₀ => forall x : El A, (B x).2 (f₀ x)).
+
+Notation "A →ᶠ B" := (Prodᶠ A (fun _ => B)) (at level 99, right associativity, B at level 200).
+Notation "'Πᶠ'  x .. y , P" := (Prodᶠ _ (fun x => .. (Prodᶠ _ (fun y => P)) ..))
+  (at level 200, x binder, y binder, right associativity).
+
+Definition Lamᶠ {A : El Tyᵗ} {B : El A -> El Tyᵗ} (f : forall x : El A, El (B x)) : El (Prodᶠ A B).
+Proof.
+unshelve refine (_ ; _).
++ refine (fun x => (f x).1).
++ refine (fun x => (f x).2).
+Defined.
+
+Notation "'λᶠ'  x .. y , t" := (Lamᶠ (fun x => .. (Lamᶠ (fun y => t)) ..))
+  (at level 200, x binder, y binder, right associativity).
+
+Definition Appᶠ {A B} (f : El (Prodᶠ A B)) (x : El A) : El (B x).
+Proof.
+unshelve refine (_ ; _).
++ refine (f.1 x).
++ refine (f.2 x).
+Defined.
+
+Notation "t · u" := (Appᶠ t u) (at level 65, left associativity).
+
+
+Definition sigmaᵀ (A : El Tyᵗ) (P : El (A →ᶠ Tyᵗ)) : Type :=
+  sigma (El A) (fun x => El (P · x)).
+
+Definition existᵀ (A : El Tyᵗ) (P : El (A →ᶠ Tyᵗ))
+           (x : El A) (y : El (P · x)) : sigmaᵀ A P
+  := mk_sig x y.
+
+Inductive sigmaᴿ (A : El Tyᵗ) (P : El (A →ᶠ Tyᵗ)) : sigmaᵀ A P -> Type :=
+| existᴿ : forall (x : El A) (y : El (P · x)), sigmaᴿ A P (existᵀ A P x y).
+
+Definition sigmaᶠ : El (Πᶠ (A : El Tyᵗ) (P : El (A →ᶠ Tyᵗ)), Tyᵗ).
+Proof.
+refine (λᶠ A P, _).
+unshelve refine (mkTYPE _ (sigmaᴿ A P)).
+Defined.
+
+Definition existᶠ : El (Πᶠ (A : El Tyᵗ) (P : El (A →ᶠ Tyᵗ)) (x : El A) (y : El (P · x)),
+  sigmaᶠ · A · P).
+Proof.
+refine (λᶠ A P x y, _).
+refine (mk_sig (existᵀ A P x y) (existᴿ A P x y)).
+Defined.
+
+
+Fixpoint extract_mind_decl_from_program (id : ident) (p : program)
+  : option minductive_decl
+  := match p with
+     | PConstr _ _ _ _ p => extract_mind_decl_from_program id p
+     | PType id' n inds p => if string_dec id id' then
+                              Some (Build_minductive_decl n inds)
+                            else extract_mind_decl_from_program id p
+     | PAxiom _ _ _ p => extract_mind_decl_from_program id p
+     | PIn _ => None
+     end.
+
+Inductive eq@{i} {A : Type@{i}} (x : A) : A -> Type@{i} :=  eq_refl : eq x x.
+
+Inductive eq2 (A : El Tyᵗ) (x : El A) :
+  forall (y : El A), eq (π1 x) (π1 y) -> Prop :=
+| refl2 : eq2 A x x (eq_refl _).
+
+
+Definition eqᶠ : El (Πᶠ (A : El Tyᵗ), A →ᶠ A →ᶠ Tyᵗ).
+Proof.
+refine (λᶠ A x y, _).
+unshelve refine (mkTYPE _ _).
++ refine (eq x.1 y.1).
++ refine (eq2 A x y).
+Defined.
+
+Definition reflᶠ : El (Πᶠ (A : El Tyᵗ) (x : El A), eqᶠ · A · x · x).
+Proof.
+refine (λᶠ A x, _).
+unshelve refine (_; refl2 A x).
+Defined.
+
+Definition Falseᶠ : El Tyᵗ.
+  exists False. exact (fun _ => False).
+Defined.
+  
+
+Quote Recursively Definition sigma_prog := @sigma.
+Quote Recursively Definition eq_prog := @eq.
+Quote Recursively Definition false_prog := @False.
+Definition sigma_decl := Eval compute in
+      extract_mind_decl_from_program "Translations.sigma.sigma" sigma_prog.
+Definition eq_decl := Eval compute in
+      extract_mind_decl_from_program "Translations.tsl_param.eq" eq_prog.
+Definition false_decl := Eval compute in
+      extract_mind_decl_from_program "Coq.Init.Logic.False" false_prog.
+
+
+Definition ΣE : option tsl_context :=
+  sd <- sigma_decl ;;
+  ed <- eq_decl ;;
+  fd <- false_decl ;;
+  let Σ' := [InductiveDecl "Coq.Init.Logic.False" fd;
+             InductiveDecl "Translations.tsl_param.eq" ed;
+             InductiveDecl "Translations.sigma.sigma" sd] in
+  let E' := [(IndRef (mkInd "Translations.sigma.sigma" 0),
+              tConst "sigmaᶠ" []);
+             (ConstructRef (mkInd "Translations.sigma.sigma" 0) 0,
+              tConst "existᶠ" []);
+             (IndRef (mkInd "Translations.tsl_param.eq" 0), tConst "eqᶠ" []);
+             (IndRef (mkInd "Coq.Init.Logic.False" 0), tConst "Falseᶠ" [])
+            ] in
+  ret (Σ', E').
+
+
+Definition HasTwoElFstComponentᵗ : El (Tyᵗ →ᶠ Tyᵗ)
+  := λᶠ (T : El Tyᵗ), mkTYPE (exists (x y : T.1), x = y -> False) (fun _ => unit).
+
+
+Definition equiv (A B : Type) :=
+  (* Type. *)
+  exists (f : A -> B) (g : B -> A),
+    (forall x, eq (g (f x)) x) × (forall x, eq (f (g x)) x).
+
+Definition FALSE := forall X, X.
+Run TemplateProgram (TslParam ([],[]) "FALSE").
+
+Proposition consistency_preservation : El FALSEᵗ -> FALSE.
+  compute.
+  intros [f _] X.
+  exact (f (X; fun _ => unit)).
+Defined.
+
+Quote Definition equiv_ := Eval compute in equiv.
+
+
+Time Definition uu := Eval native_compute in (tsl_tm (match ΣE with Some ΣE => ΣE | None => todo end) equiv_).
+Time Definition uu' := Eval native_compute in (tsl_tm (match ΣE with Some ΣE => ΣE | None => todo end) equiv_).
+
+Time Eval native_compute in (tsl_tm (match ΣE with Some ΣE => ΣE | None => todo end) equiv_).
+
+Print "go".
+
+Run TemplateProgram (
+      match ΣE with
+      | None => tmPrint "li" ;; tmReturn None
+      | Some ΣE =>
+        ΣE' <- TslParam ΣE "equiv" ;;
+            tmPrint ΣE' ;;
+            match ΣE' with
+            | None => tmReturn None
+            | Some ΣE =>
+              tmPrint "lo" ;;
+              H <- ImplParam ΣE "notUnivalence"
+              (exists A B : Type, (equiv A B) × exists P, P A × ((P B) -> False)) ;;
+              (* (exists A : Type, (equiv A A)) ;; *)
+              tmPrint "la" ;; ret H
+            end
+      end).
+Next Obligation.
+simple refine (existᶠ · _ · _ · _ · _).
+exact (bool:Type; fun _=> unit:Type).
+simple refine (existᶠ · _ · _ · _ · _).
+exact (unit:Type; fun _ => bool:Type).
+simple refine (existᶠ · _ · _ · _ · _).
+- simple refine (existᶠ · _ · _ · _ · _).
+  exists π2. exact π1.
+  simple refine (existᶠ · _ · _ · _ · _).
+  exists π2. exact π1.
+  simple refine (existᶠ · _ · _ · _ · _);
+    cbn; unshelve econstructor; reflexivity.
+- simple refine (existᶠ · _ · _ · _ · _).
+  exact HasTwoElFstComponentᵗ.
+  simple refine (existᶠ · _ · _ · _ · _).
+  + cbn. refine (_; tt). exists true. exists false.
+    discriminate 1.
+  + refine (λᶠ p, _). cbn in p.
+    destruct p as [p _].
+    destruct p as [[] [[] p]].
+    contradiction p. reflexivity.
+Defined.
+
+Print "ok!".
